LeanSAT/Reflect/BVExpr/BitBlast/Lemmas/SignExtend.lean
@@ -1,0 +1,104 @@
+import LeanSAT.Reflect.BVExpr.BitBlast.Lemmas.Basic
+import LeanSAT.Reflect.BVExpr.BitBlast.Lemmas.ZeroExtend
+import LeanSAT.Reflect.BVExpr.BitBlast.Impl.SignExtend
+
+open AIG
+
+theorem signExtend_eq_neg_zeroExtend_neg_of_msb_false {x : BitVec w} {v : Nat} (hmsb : x.msb = false) :
+    (x.signExtend v) = x.zeroExtend v := by
+  sorry
+
+theorem getLsb_signExtend (x  : BitVec w) {v i : Nat} :
+    (x.signExtend v).getLsb i = (decide (i < v) && if i < w then x.getLsb i else x.msb) := by
+  sorry
+
+namespace BVExpr
+namespace bitblast
+namespace blastSignExtend
+
+theorem go_getRef_aux (aig : AIG BVBit) (w : Nat) (hw : 0 < w) (input : RefStream aig w) (newWidth : Nat)
+    (curr : Nat) (hcurr : curr ≤ newWidth) (s : RefStream aig curr)
+    : ∀ (idx : Nat) (hidx1 : idx < curr),
+        (go w hw input newWidth curr hcurr s).getRef idx (by omega)
+          =
+        s.getRef idx hidx1 := by
+  intro idx hidx
+  unfold go
+  split
+  . dsimp
+    split
+    all_goals
+      rw [go_getRef_aux]
+      rw [AIG.RefStream.getRef_push_ref_lt]
+  . dsimp
+    simp only [RefStream.getRef, Ref.mk.injEq]
+    congr
+    . omega
+    . simp
+
+theorem go_getRef (aig : AIG BVBit) (w : Nat) (hw : 0 < w) (input : RefStream aig w) (newWidth : Nat)
+    (curr : Nat) (hcurr : curr ≤ newWidth) (s : RefStream aig curr)
+    : ∀ (idx : Nat) (hidx1 : idx < newWidth),
+        curr ≤ idx
+          →
+        (go w hw input newWidth curr hcurr s).getRef idx hidx1
+          =
+        if hidx2:idx < w then
+          input.getRef idx (by omega)
+        else
+          input.getRef (w - 1) (by omega)
+    := by
+  intro idx hidx1 hcurr
+  unfold go
+  have : curr < newWidth := by omega
+  simp only [this, ↓reduceDite]
+  cases Nat.eq_or_lt_of_le hcurr with
+  | inl heq =>
+    simp only [heq]
+    split
+    all_goals
+      rw [go_getRef_aux]
+      rw [AIG.RefStream.getRef_push_ref_eq']
+      rw [heq]
+  | inr heq =>
+    split
+    all_goals
+      rw [go_getRef]
+      omega
+
+end blastSignExtend
+
+theorem blastSignExtend_empty_eq_zeroExtend (aig : AIG BVBit) (target : ExtendTarget aig newWidth)
+      (htarget : target.w = 0)
+  : blastSignExtend aig target = blastZeroExtend aig target := by
+  unfold blastSignExtend
+  simp [htarget]
+
+theorem blastSignExtend_eq_eval_getLsb (aig : AIG BVBit) (target : ExtendTarget aig newWidth)
+  (assign : Assignment) (htarget : 0 < target.w)
+  : ∀ (idx : Nat) (hidx : idx < newWidth),
+      ⟦
+        (blastSignExtend aig target).aig,
+        (blastSignExtend aig target).stream.getRef idx hidx,
+        assign.toAIGAssignment
+      ⟧
+        =
+      if hidx:idx < target.w then
+         ⟦aig, target.stream.getRef idx hidx, assign.toAIGAssignment⟧
+      else
+         ⟦aig, target.stream.getRef (target.w - 1) (by omega), assign.toAIGAssignment⟧
+    := by
+  intro idx hidx
+  generalize hg : blastSignExtend aig target = res
+  unfold blastSignExtend at hg
+  dsimp at hg
+  have : ¬ (target.w = 0) := by omega
+  simp only [this, ↓reduceDite] at hg
+  rw [← hg]
+  dsimp
+  rw [blastSignExtend.go_getRef]
+  . split <;> simp only
+  . omega
+
+end bitblast
+end BVExpr
